\begin{frame}[t]

	\frametitle{Raising a number to an Imaginary power}

	If we let \(n = 1\), then we have;\\~
	\begin{equation} \label{eqn_slide_10_a}
	e^{j}
	\end{equation}

	The result of this is that \(e\) gets multiplied by \(j\) once. That is;
	\begin{equation} \label{eqn_slide_10_b}
	e^{j} = j \times e
	\end{equation}

	Similarly;
	\begin{align} \label{eqn_slide_10_c}
	e^{j2} &= j \times j \times e \\
	e^{j3} &= j \times j \times j \times e \\
	e^{j4} &= j \times j \times j \times j \times e
	\end{align}

\end{frame}
